Coq/src/Example.v
@@ -12,335 +12,365 @@ Definition coin := Coin__Bool.
 Definition share := Share.
 Definition const := fun A (x _ : A) => x.
 
-Example example1 : Prog bool := coin.
-Example res_example1 := [true; false].
+Section exB.
+  Example example1 : Prog bool := coin.
+  Example res_example1 := [true; false].
 
-Example example2 : Prog bool := coin ? coin.
-Example res_example2 := [true; false; true; false].
+  Example example2 : Prog bool := coin ? coin.
+  Example res_example2 := [true; false; true; false].
+  
+  Example example3 : Prog bool :=  share coin >>= fun fx => fx ? fx.
+  Example res_example3 := res_example2.
+  
+  Example exOr0 : Prog bool := orM coin (pure false).
+  Example res_exOr0 := [true; false].
+  
+  Example exOr1 : Prog bool := orM coin coin.
+  Example res_exOr1 := [true; true; false].
+  
+  Example exOr2 : Prog bool := share coin >>= fun fx => orM fx fx.
+  Example res_exOr2 := [true; false].
+  
+  Example exOr2a : Prog bool :=
+    share coin >>= fun fx => orM (pure false) (orM fx fx).
+  Example res_exOr2a := [true; false].
+  
+  Example exOr2b : Prog bool :=
+    share coin >>= fun fx => orM (pure true) (orM fx fx).
+  Example res_exOr2b := [true].
+  
+  Example exOr3 : Prog bool := orM (coin ? coin) (pure true).
+  Example res_exOr3 := [true; true; true; true].
+  
+  Example exOr3a : Prog bool := orM (coin ? coin) coin.
+  Example res_exOr3a := [true; true; false; true; true; false].
+  
+  Example exOr3b : Prog bool := orM coin (coin ? coin).
+  Example res_exOr3b := [true; true; false; true; false].
+  
+  Example exOr3c : Prog bool := orM (coin ? coin) (coin ? coin).
+  Example res_exOr3c := [true; true; false; true; false; true; true; false; true; false].
+  
+  (* here we share, even though nothing is shared *)
+  Example exOr4 : Prog bool := share coin >>= fun fx => orM fx coin.
+  Example res_exOr4 := [true; true; false].
+  
+  Example exOrShare : Prog bool := share coin >>= fun fx => orM coin fx.
+  Example res_exOrShare := [true; true; false].
+  
+  Example exOr6 : Prog bool := share coin >>= fun fx => orM fx (orM fx coin).
+  Example res_exOr6 := [true; true; false].
+  
+  Example exOr7 : Prog bool := share coin >>= fun fx => orM coin (orM fx fx).
+  Example res_exOr7 := [true; true; false].
+  
+  Example exOr7a : Prog bool := share coin >>= fun fx => orM (pure true) (orM fx fx).
+  Example res_exOr7a := [true].
+  
+  Example exOr7b : Prog bool := share coin >>= fun fx => orM (pure false) (orM fx fx).
+  Example res_exOr7b := [true; false].
+  
+  Example exShareConst : Prog bool := share coin >>= fun fx => const fx fx.
+  Example res_exShareConst := [true; false].
+  
+  Example exShareConstOrR : Prog bool := share coin >>= fun fx => orM fx (const fx fx).
+  Example res_exShareConstOrR := [true; false].
+  
+  Example exShareConstOrL : Prog bool := share coin >>= fun fx => orM (const fx fx) fx.
+  Example res_exShareConstOrL := [true; false].
+  
+  Example exShareConstOrR2 : Prog bool := share coin >>= fun fx => orM (pure true) (const fx fx).
+  Example res_exShareConstOrR2 := [true].
+  
+  Example exFailed : Prog bool := share Fail >>= fun fx => const (pure true) fx.
+  Example res_exFailed := [true].
+  
+  Example exHead : Prog bool := headM (consM coin Fail).
+  Example res_exHead := [true; false].
+  
+  Example exOrShareShare : Prog bool :=
+    share coin >>=
+          fun fx =>
+            share coin >>=
+                  fun fy =>
+                    orM fx (orM fy (orM fx fy)).
+  Example res_exOrShareShare := [true; true; false].
+  
+  Example exOrShareNested : Prog bool :=
+    share coin >>= fun fx =>
+                     orM fx (share coin >>= fun fy =>
+                                              orM fy (orM fx fy)).
+  Example res_exOrShareNested := [true; true; false].
+  
+  Example exShareNestedChoiceOr : Prog bool :=
+    share ((pure true ? pure false) ? (pure true ? pure false)) >>=
+          fun fx => orM fx fx.
+  Example res_exShareNestedChoiceOr := [true; false; true; false].
+  
+  Example exShareIgnoreShare : Prog bool :=
+    share coin >>= fun fx => const (pure true) (share fx >>= fun fy => orM fy fy).
+  Example res_exShareIgnoreShare := [true].
+  
+  Example exRepeatedShare : Prog bool :=
+    share coin >>= fun fx => share fx >>= fun fy => orM fy fy.
+  Example res_exRepeatedShare := [true; false].
+  
+  Definition exBs := [(example1, res_example1);
+                        (example2, res_example2);
+                        (example3, res_example3);
+                        (exOr0, res_exOr0);
+                        (exOr1, res_exOr1);
+                        (exOr2, res_exOr2);
+                        (exOr2a, res_exOr2a);
+                        (exOr2b, res_exOr2b);
+                        (exOr3, res_exOr3);
+                        (exOr3a, res_exOr3a);
+                        (exOr3b, res_exOr3b);
+                        (exOr3c, res_exOr3c);
+                        (exOr4, res_exOr4);
+                        (exOrShare, res_exOrShare);
+                        (exOr6, res_exOr6);
+                        (exOr7, res_exOr7);
+                        (exOr7a, res_exOr7a);
+                        (exOr7b, res_exOr7b);
+                        (exShareConst, res_exShareConst);
+                        (exShareConstOrR, res_exShareConstOrR);
+                        (exShareConstOrL, res_exShareConstOrL);
+                        (exShareConstOrR2, res_exShareConstOrR2);
+                        (exFailed, res_exFailed);
+                        (exHead, res_exHead);
+                        (exOrShareShare, res_exOrShareShare);
+                        (exOrShareNested, res_exOrShareNested);
+                        (exShareNestedChoiceOr, res_exShareNestedChoiceOr);
+                        (exShareIgnoreShare, res_exShareIgnoreShare);
+                        (exRepeatedShare, res_exRepeatedShare)].
+  
+  Lemma tests__exBs : Forall (fun '(p,r) => handle p = r) exBs.
+  Proof. repeat econstructor. Qed.
+End exB.
 
-Example example3 : Prog bool :=  share coin >>= fun fx => fx ? fx.
-Example res_example3 := res_example2.
+Section exPB.
+  Example exDup : Prog (Pair bool bool) := dup coin.
+  Example res_exDup := [Pair' (pure true) (pure true)
+                        ; Pair' (pure true) (pure false)
+                        ; Pair' (pure false) (pure true)
+                        ; Pair' (pure false) (pure false)].
+  
+  Example exDupShare : Prog (Pair bool bool) := share coin >>= fun x => dup x.
+  Example res_exDupShare := [Pair' (pure true) (pure true)
+                             ; Pair' (pure false) (pure false)].
+  
+  Example exDupShare2 : Prog (Pair bool bool) := dupShare coin.
+  Example res_exDupShare2 := [Pair' (pure true) (pure true)
+                              ; Pair' (pure false) (pure false)].
+  
+  Example exDupFailed : Prog (Pair bool bool) := share Fail >>= fun x => dup (const (pure true) x).
+  Example res_exDupFailed := [Pair' (pure true) (pure true)].
+  
+  Example exDupFirst : Prog (Pair bool bool) := dup (@first bool bool (pairM coin Fail)).
+  Example res_exDupFirst := [Pair' (pure true) (pure true)
+                             ; Pair' (pure true) (pure false)
+                             ; Pair' (pure false) (pure true)
+                             ; Pair' (pure false) (pure false)].
+  
+  Example exDupShareFirst : Prog (Pair bool bool) := dupShare (@first bool bool (pairM coin Fail)).
+  Example res_exDupShareFirst :=  [Pair' (pure true) (pure true); Pair' (pure false) (pure false)].
+  
+  Example exShareNestedChoice : Prog (Pair bool bool) :=
+    share ((pure true ? pure false) ? (pure true ? pure false)) >>=
+          fun fx => pairM fx fx.
+  Example res_exShareNestedChoice := [Pair' (pure true) (pure true) 
+                                      ; Pair' (pure false) (pure false)
+                                      ; Pair' (pure true) (pure true)
+                                      ; Pair' (pure false) (pure false)].
+  
+  Definition exPBs := [(exDup, res_exDup)
+                       ; (exDupShare, res_exDupShare)
+                       ; (exDupShare2, res_exDupShare2)
+                       ; (exDupFailed, res_exDupFailed)
+                       ; (exDupFirst, res_exDupFirst)
+                       ; (exDupShareFirst, res_exDupShareFirst)
+                       ; (exShareNestedChoice, res_exShareNestedChoice)].
+  
+  Lemma tests__exPBs : Forall (fun '(p,r) => handle p = r) exPBs.
+  Proof. repeat econstructor. Qed.
+End exPB.
 
-Example exOr0 : Prog bool := orM coin (pure false).
-Example res_exOr0 := [true; false].
+Arguments nilM {_}.
 
-Example exOr1 : Prog bool := orM coin coin.
-Example res_exOr1 := [true; true; false].
-
-Example exOr2 : Prog bool := share coin >>= fun fx => orM fx fx.
-Example res_exOr2 := [true; false].
-
-Example exOr2a : Prog bool :=
-  share coin >>= fun fx => orM (pure false) (orM fx fx).
-Example res_exOr2a := [true; false].
-
-Example exOr2b : Prog bool :=
-  share coin >>= fun fx => orM (pure true) (orM fx fx).
-Example res_exOr2b := [true].
-
-Example exOr3 : Prog bool := orM (coin ? coin) (pure true).
-Example res_exOr3 := [true; true; true; true].
-
-Example exOr3a : Prog bool := orM (coin ? coin) coin.
-Example res_exOr3a := [true; true; false; true; true; false].
-
-Example exOr3b : Prog bool := orM coin (coin ? coin).
-Example res_exOr3b := [true; true; false; true; false].
-
-Example exOr3c : Prog bool := orM (coin ? coin) (coin ? coin).
-Example res_exOr3c := [true; true; false; true; false; true; true; false; true; false].
-
-(* here we share, even though nothing is shared *)
-Example exOr4 : Prog bool := share coin >>= fun fx => orM fx coin.
-Example res_exOr4 := [true; true; false].
-
-Example exOrShare : Prog bool := share coin >>= fun fx => orM coin fx.
-Example res_exOrShare := [true; true; false].
-
-Example exOr6 : Prog bool := share coin >>= fun fx => orM fx (orM fx coin).
-Example res_exOr6 := [true; true; false].
-
-Example exOr7 : Prog bool := share coin >>= fun fx => orM coin (orM fx fx).
-Example res_exOr7 := [true; true; false].
-
-Example exOr7a : Prog bool := share coin >>= fun fx => orM (pure true) (orM fx fx).
-Example res_exOr7a := [true].
-
-Example exOr7b : Prog bool := share coin >>= fun fx => orM (pure false) (orM fx fx).
-Example res_exOr7b := [true; false].
-
-Example exShareConst : Prog bool := share coin >>= fun fx => const fx fx.
-Example res_exShareConst := [true; false].
-
-Example exShareConstOrR : Prog bool := share coin >>= fun fx => orM fx (const fx fx).
-Example res_exShareConstOrR := [true; false].
-
-Example exShareConstOrL : Prog bool := share coin >>= fun fx => orM (const fx fx) fx.
-Example res_exShareConstOrL := [true; false].
-
-Example exShareConstOrR2 : Prog bool := share coin >>= fun fx => orM (pure true) (const fx fx).
-Example res_exShareConstOrR2 := [true].
-
-Example exFailed : Prog bool := share Fail >>= fun fx => const (pure true) fx.
-Example res_exFailed := [true].
-
-Example exHead : Prog bool := headM (consM coin Fail).
-Example res_exHead := [true; false].
-
-Example exOrShareShare : Prog bool :=
-  share coin >>=
-        fun fx =>
-          share coin >>=
-                fun fy =>
-                  orM fx (orM fy (orM fx fy)).
-Example res_exOrShareShare := [true; true; false].
-
-Example exOrShareNested : Prog bool :=
+Example exOrShareNestedList : Prog (List bool) :=
   share coin >>= fun fx =>
-                   orM fx (share coin >>= fun fy =>
-                                            orM fy (orM fx fy)).
-Example res_exOrShareNested := [true; true; false].
-
-Example exShareNestedChoiceOr : Prog bool :=
-  share ((pure true ? pure false) ? (pure true ? pure false)) >>=
-        fun fx => orM fx fx.
-Example res_exShareNestedChoiceOr := [true; false; true; false].
-
-Example exShareIgnoreShare : Prog bool :=
-  share coin >>= fun fx => const (pure true) (share fx >>= fun fy => orM fy fy).
-Example res_exShareIgnoreShare := [true].
-
-Example exRepeatedShare : Prog bool :=
-  share coin >>= fun fx => share fx >>= fun fy => orM fy fy.
-Example res_exRepeatedShare := [true; false].
-
-Definition exBs := [(example1, res_example1);
-                      (example2, res_example2);
-                      (example3, res_example3);
-                      (exOr0, res_exOr0);
-                      (exOr1, res_exOr1);
-                      (exOr2, res_exOr2);
-                      (exOr2a, res_exOr2a);
-                      (exOr2b, res_exOr2b);
-                      (exOr3, res_exOr3);
-                      (exOr3a, res_exOr3a);
-                      (exOr3b, res_exOr3b);
-                      (exOr3c, res_exOr3c);
-                      (exOr4, res_exOr4);
-                      (exOrShare, res_exOrShare);
-                      (exOr6, res_exOr6);
-                      (exOr7, res_exOr7);
-                      (exOr7a, res_exOr7a);
-                      (exOr7b, res_exOr7b);
-                      (exShareConst, res_exShareConst);
-                      (exShareConstOrR, res_exShareConstOrR);
-                      (exShareConstOrL, res_exShareConstOrL);
-                      (exShareConstOrR2, res_exShareConstOrR2);
-                      (exFailed, res_exFailed);
-                      (exHead, res_exHead);
-                      (exOrShareShare, res_exOrShareShare);
-                      (exOrShareNested, res_exOrShareNested);
-                      (exShareNestedChoiceOr, res_exShareNestedChoiceOr);
-                      (exShareIgnoreShare, res_exShareIgnoreShare);
-                      (exRepeatedShare, res_exRepeatedShare)].
-                      
-Lemma tests__exBs : Forall (fun '(p,r) => handle p = r) exBs.
-Proof. repeat econstructor. Qed.
+                   consM fx (share coin >>= fun fy =>
+                                             consM fy (consM fx (consM fy nilM))).
 (*
-exOrShareNestedList :: (Sharing m, MonadPlus m) => m (List m Bool)
-exOrShareNestedList = share coin >>= \fx ->
-                  cons fx (share coin >>= \fy ->
-                              cons fy (cons fx (cons fy nil)))
-
-recList :: (Sharing m, MonadPlus m) => m (List m Bool) -> m (List m Bool)
-recList fxs = fxs >>= \xfps -> case xfps of
-                                    Nil -> nil
-                                    Cons fy fys -> share fys >>= \fys' -> cons fy (fys' `mplus` recList fys')
+recList :: (Sharing m, MonadPlus m) => m (List m Bool) => m (List m Bool)
+recList fxs = fxs >>= fun xfps => case xfps of
+                                    Nil' => nil
+                                    Cons' fy fys => share fys >>= fun fys' => consM fy (fys' `mplus` recList fys')
 
 exRecList :: (Sharing m, MonadPlus m) => m (Pair m (List m Bool))
-exRecList = share (recList (cons (return True) (cons (return False) nil))) >>= \fx -> pairM fx fx
+exRecList = share (recList (consM (pure true) (consM (pure false) nil))) >>= fun fx => pairM fx fx
 
 exRecListNested :: (Sharing m, MonadPlus m) => m (List m (List m Bool))
-exRecListNested = share (recList (cons (return True) (cons (return False) nil)))
-  >>= \fx -> cons fx (share (recList (cons (return True) (cons (return False) nil)))
-                      >>= \fz -> cons fz (cons fx (cons fz nil)))
+exRecListNested = share (recList (consM (pure true) (consM (pure false) nil)))
+  >>= fun fx => consM fx (share (recList (consM (pure true) (consM (pure false) nil)))
+                      >>= fun fz => consM fz (consM fx (consM fz nil)))
 exSkipIds :: (Sharing m, MonadPlus m) => m Bool
-exSkipIds = share coin >>= \fx -> const coin (const fx fx)
+exSkipIds = share coin >>= fun fx => const coin (const fx fx)
 exLoop :: Sharing m => m Bool
 exLoop = let loop :: m ()
-             loop = loop in share loop >>= \fx -> const (return True) (const fx fx)
+             loop = loop in share loop >>= fun fx => const (pure true) (const fx fx)
 exLoop2 :: Sharing m => m Bool
 exLoop2 = let loop :: m ()
-              loop = loop in share loop >>= \fx -> const coin (const fx fx)
-
-exDup :: (Sharing m, MonadPlus m) => m (Pair m Bool)
-exDup = dup coin
-exDupShare :: (Sharing m, MonadPlus m) => m (Pair m Bool)
-exDupShare = share coin >>= dup
-exDupShare2 :: (Sharing m, MonadPlus m) => m (Pair m Bool)
-exDupShare2 = dupShare coin
-exDupFailed :: (Sharing m, MonadPlus m) => m (Pair m Bool)
-exDupFailed = share (mzero :: MonadPlus m => m Bool) >>= \x -> dup (const (return True) x)
-exDupFirst :: MonadPlus m => m (Pair m Bool)
-exDupFirst = dup (first (pairM coin mzero))
-exDupShareFirst :: (Sharing m, MonadPlus m) => m (Pair m Bool)
-exDupShareFirst = dupShare (first (pairM coin mzero))
+              loop = loop in share loop >>= fun fx => const coin (const fx fx)
 
 exDupl :: MonadPlus m => m (List m Bool)
-exDupl = dupl (headM (cons coin (mzero :: MonadPlus m => m (List m Bool))))
+exDupl = dupl (headM (consM coin (mzero :: MonadPlus m => m (List m Bool))))
 exDupl2 :: MonadPlus m => m (List m Bool)
-exDupl2 = cons (headM (cons coin (mzero :: MonadPlus m => m (List m Bool))))
-               (cons (headM (cons coin (mzero :: MonadPlus m => m (List m Bool))))
+exDupl2 = consM (headM (consM coin (mzero :: MonadPlus m => m (List m Bool))))
+               (consM (headM (consM coin (mzero :: MonadPlus m => m (List m Bool))))
                      nil)
 exDuplShare :: (Sharing m, MonadPlus m) => m (List m Bool)
-exDuplShare = duplShare (headM (cons coin (mzero :: MonadPlus m => m (List m Bool))))
-
-exShareNestedChoice :: (Sharing m, MonadPlus m) => m (Pair m Bool)
-exShareNestedChoice =
-  share (mplus (mplus (return True) (return False)) (mplus (return True) (return False))) >>=
-    \fx -> pairM fx fx
-
+exDuplShare = duplShare (headM (consM coin (mzero :: MonadPlus m => m (List m Bool))))
 
 exShareNestedChoice2 :: (Sharing m, MonadPlus m) => m (List m Bool)
 exShareNestedChoice2 =
-  share (mplus (return True) (mplus (return False) (return True))) >>=
-    \fx -> share (mplus (return True) (return False)) >>= \fy -> cons fx (cons fy (cons fx (cons fy nil)))
+  share (mplus (pure true) (mplus (pure false) (pure true))) >>=
+    fun fx => share (mplus (pure true) (pure false)) >>= fun fy => consM fx (consM fy (consM fx (consM fy nil)))
 
 
 exShareSingleton :: (Sharing m, MonadPlus m) => m (Pair m (List m Bool))
 exShareSingleton =
-  share (cons (return True `mplus` return False) nil) >>=
-    \fx -> pairM fx fx
+  share (consM (pure true `mplus` pure false) nil) >>=
+    fun fx => pairM fx fx
 
 exShareInShare :: (Sharing m, MonadPlus m) => m (Pair m Bool)
-exShareInShare = share (share coin >>= \fx -> orM fx fx) >>= \fy -> pairM fy fy
+exShareInShare = share (share coin >>= fun fx => orM fx fx) >>= fun fy => pairM fy fy
 
 exShareListInShare :: (Sharing m, MonadPlus m) => m (Pair m (List m Bool))
 exShareListInShare =
-  share (share (cons coin (cons coin nil)) >>=
-          \fx -> appM fx fx) >>= \fy -> pairM fy fy
+  share (share (consM coin (consM coin nil)) >>=
+          fun fx => appM fx fx) >>= fun fy => pairM fy fy
 
 exSharePutPos :: (Sharing m, MonadPlus m) =>  m (List m Bool)
 exSharePutPos =
-  share (share (cons coin nil) >>= \fx -> appM fx fx) >>= \fy -> appM fy fy
+  share (share (consM coin nil) >>= fun fx => appM fx fx) >>= fun fy => appM fy fy
 
 exShareListInRepeatedShare :: NDShare (List NDShare Bool)
 exShareListInRepeatedShare =
-  share (share (cons coin nil) >>= \fx -> appM fx fx) >>=
-  \fy -> share coin >>= \fz -> share coin >>= \fa -> cons fz (cons fa fy)
+  share (share (consM coin nil) >>= fun fx => appM fx fx) >>=
+  fun fy => share coin >>= fun fz => share coin >>= fun fa => consM fz (consM fa fy)
 
 tests = do
-  let exBs  = [ (example1,"ex1",[True,False])
-              , (example2,"ex2",[True,False,True,False])
-              , (example3,"ex3",[True,False,True,False])
-              , (exOr0,"exOr0",[True,False])
-              , (exOr1,"exOr1",[True,True,False])
-              , (exOr2,"exOr2",[True,False])
-              , (exOr2a,"exOr2a",[True,False])
-              , (exOr2b,"exOr2b",[True])
-              , (exOr3,"exOr3",[True,True,True,True])
-              , (exOr3a,"exOr3a",[True,True,False,True,True,False])
-              , (exOr3b,"exOr3b",[True,True,False,True,False])
-              , (exOr3c,"exOr3c",[True,True,False,True,False,True,True,False,True,False])
-              , (exOr4,"exOr4",[True,True,False])
-              , (exOrShare,"exOrShare",[True,True,False])
-              , (exOr6,"exOr6",[True,True,False])
-              , (exOr7,"exOr7",[True,True,False])
-              , (exOr7a,"exOr7a",[True])
-              , (exOr7b,"exOr7b",[True,False])
-              , (exShareConst,"exShareConst",[True,False])
-              , (exShareConstOrR,"exShareConstOrR",[True,False])
-              , (exShareConstOrL,"exShareConstOrL",[True,False])
-              , (exShareConstOrR2,"exShareConstOrR2",[True])
-              , (exFailed,"exFailed",[True])
-              , (exHead,"exHead", [ True, False ])
-              , (exOrShareShare,"exOrShareShare", [True,True,False])
-              , (exOrShareNested,"exOrShareNested", [True,True,False])
-              , (exShareNestedChoiceOr, "exShareNestedChoiceOr", [True,False,True,False])
-              , (exShareIgnoreShare, "exShareIgnoreShare", [True])
-              , (exRepeatedShare, "exRepeatedShare", [True,False])
+  let exBs  = [ (example1,"ex1",[true,false])
+              , (example2,"ex2",[true,false,true,false])
+              , (example3,"ex3",[true,false,true,false])
+              , (exOr0,"exOr0",[true,false])
+              , (exOr1,"exOr1",[true,true,false])
+              , (exOr2,"exOr2",[true,false])
+              , (exOr2a,"exOr2a",[true,false])
+              , (exOr2b,"exOr2b",[true])
+              , (exOr3,"exOr3",[true,true,true,true])
+              , (exOr3a,"exOr3a",[true,true,false,true,true,false])
+              , (exOr3b,"exOr3b",[true,true,false,true,false])
+              , (exOr3c,"exOr3c",[true,true,false,true,false,true,true,false,true,false])
+              , (exOr4,"exOr4",[true,true,false])
+              , (exOrShare,"exOrShare",[true,true,false])
+              , (exOr6,"exOr6",[true,true,false])
+              , (exOr7,"exOr7",[true,true,false])
+              , (exOr7a,"exOr7a",[true])
+              , (exOr7b,"exOr7b",[true,false])
+              , (exShareConst,"exShareConst",[true,false])
+              , (exShareConstOrR,"exShareConstOrR",[true,false])
+              , (exShareConstOrL,"exShareConstOrL",[true,false])
+              , (exShareConstOrR2,"exShareConstOrR2",[true])
+              , (exFailed,"exFailed",[true])
+              , (exHead,"exHead", [ true, false ])
+              , (exOrShareShare,"exOrShareShare", [true,true,false])
+              , (exOrShareNested,"exOrShareNested", [true,true,false])
+              , (exShareNestedChoiceOr, "exShareNestedChoiceOr", [true,false,true,false])
+              , (exShareIgnoreShare, "exShareIgnoreShare", [true])
+              , (exRepeatedShare, "exRepeatedShare", [true,false])
               ]
-      exPBs = [ (exDup,"exDup",[ Pair (Identity True) (Identity True)
-                               , Pair (Identity True) (Identity False)
-                               , Pair (Identity False) (Identity True)
-                               , Pair (Identity False) (Identity False)
+      exPBs = [ (exDup,"exDup",[ Pair (Identity true) (Identity true)
+                               , Pair (Identity true) (Identity false)
+                               , Pair (Identity false) (Identity true)
+                               , Pair (Identity false) (Identity false)
                                ])
-              , (exDupShare,"exDupShare",[ Pair (Identity True) (Identity True)
-                                         , Pair (Identity False) (Identity False)
+              , (exDupShare,"exDupShare",[ Pair (Identity true) (Identity true)
+                                         , Pair (Identity false) (Identity false)
                                          ])
-              , (exDupShare2,"exDupShare2",[ Pair (Identity True) (Identity True)
-                                           , Pair (Identity False) (Identity False)
+              , (exDupShare2,"exDupShare2",[ Pair (Identity true) (Identity true)
+                                           , Pair (Identity false) (Identity false)
                                            ])
-              , (exDupFailed,"exDupFailed",[ Pair (Identity True) (Identity True) ])
-              , (exDupFirst,"exDupFirst",[ Pair (Identity True) (Identity True)
-                                         , Pair (Identity True) (Identity False)
-                                         , Pair (Identity False) (Identity True)
-                                         , Pair (Identity False) (Identity False)
+              , (exDupFailed,"exDupFailed",[ Pair (Identity true) (Identity true) ])
+              , (exDupFirst,"exDupFirst",[ Pair (Identity true) (Identity true)
+                                         , Pair (Identity true) (Identity false)
+                                         , Pair (Identity false) (Identity true)
+                                         , Pair (Identity false) (Identity false)
                                          ])
-              , (exDupShareFirst,"exShareDupFirst", [ Pair (Identity True) (Identity True)
-                                                    , Pair (Identity False) (Identity False)
+              , (exDupShareFirst,"exShareDupFirst", [ Pair (Identity true) (Identity true)
+                                                    , Pair (Identity false) (Identity false)
                                                     ])
-              , (exDupShare2,"exDupShare2",[ Pair (Identity True) (Identity True)
-                                           , Pair (Identity False) (Identity False)
+              , (exDupShare2,"exDupShare2",[ Pair (Identity true) (Identity true)
+                                           , Pair (Identity false) (Identity false)
                                            ])
               , (exShareNestedChoice, "exShareNestedChoice",
-                               [ Pair (Identity True) (Identity True)
-                               , Pair (Identity False) (Identity False)
-                               , Pair (Identity True) (Identity True)
-                               , Pair (Identity False) (Identity False)
+                               [ Pair (Identity true) (Identity true)
+                               , Pair (Identity false) (Identity false)
+                               , Pair (Identity true) (Identity true)
+                               , Pair (Identity false) (Identity false)
                                ])
               ]
-      exLBs = [ (exDupl,"exDupl", [ Cons (Identity True) (cons (Identity True) nil)
-                                    , Cons (Identity True) (cons (Identity False) nil)
-                                    , Cons (Identity False) (cons (Identity True) nil)
-                                    , Cons (Identity False) (cons (Identity False) nil)
+      exLBs = [ (exDupl,"exDupl", [ ConsM (Identity true) (consM (Identity true) nil)
+                                    , ConsM (Identity true) (consM (Identity false) nil)
+                                    , ConsM (Identity false) (consM (Identity true) nil)
+                                    , ConsM (Identity false) (consM (Identity false) nil)
                                     ])
-              , (exDuplShare,"exDuplShare", [ Cons (Identity True) (cons (Identity True) nil)
-                                            , Cons (Identity False) (cons (Identity False) nil)
+              , (exDuplShare,"exDuplShare", [ ConsM (Identity true) (consM (Identity true) nil)
+                                            , ConsM (Identity false) (consM (Identity false) nil)
                                             ])
-              , (exDupl2,"exDupl2", [ Cons (Identity True) (cons (Identity True) nil)
-                                    , Cons (Identity True) (cons (Identity False) nil)
-                                    , Cons (Identity False) (cons (Identity True) nil)
-                                    , Cons (Identity False) (cons (Identity False) nil)
+              , (exDupl2,"exDupl2", [ ConsM (Identity true) (consM (Identity true) nil)
+                                    , ConsM (Identity true) (consM (Identity false) nil)
+                                    , ConsM (Identity false) (consM (Identity true) nil)
+                                    , ConsM (Identity false) (consM (Identity false) nil)
                                     ])
               , (exShareNestedChoice2, "exShareNestedChoice2",
-                  [ Cons (Identity True) (cons (Identity True) (cons (Identity True) (cons (Identity True) nil)))
-                  , Cons (Identity True) (cons (Identity False) (cons (Identity True) (cons (Identity False) nil)))
-                  , Cons (Identity False) (cons (Identity True) (cons (Identity False) (cons (Identity True) nil)))
-                  , Cons (Identity False) (cons (Identity False) (cons (Identity False) (cons (Identity False) nil)))
-                  , Cons (Identity True) (cons (Identity True) (cons (Identity True) (cons (Identity True) nil)))
-                  , Cons (Identity True) (cons (Identity False) (cons (Identity True) (cons (Identity False) nil)))
+                  [ ConsM (Identity true) (consM (Identity true) (consM (Identity true) (consM (Identity true) nil)))
+                  , ConsM (Identity true) (consM (Identity false) (consM (Identity true) (consM (Identity false) nil)))
+                  , ConsM (Identity false) (consM (Identity true) (consM (Identity false) (consM (Identity true) nil)))
+                  , ConsM (Identity false) (consM (Identity false) (consM (Identity false) (consM (Identity false) nil)))
+                  , ConsM (Identity true) (consM (Identity true) (consM (Identity true) (consM (Identity true) nil)))
+                  , ConsM (Identity true) (consM (Identity false) (consM (Identity true) (consM (Identity false) nil)))
                   ])
               , (exOrShareNestedList, "exOrShareNestedList",
-                 [ Cons (Identity True) (cons (Identity True) (cons (Identity True) (cons (Identity True) nil)))
-                 , Cons (Identity True) (cons (Identity False) (cons (Identity True) (cons (Identity False) nil)))
-                 , Cons (Identity False) (cons (Identity True) (cons (Identity False) (cons (Identity True) nil)))
-                 , Cons (Identity False) (cons (Identity False) (cons (Identity False) (cons (Identity False) nil)))
+                 [ ConsM (Identity true) (consM (Identity true) (consM (Identity true) (consM (Identity true) nil)))
+                 , ConsM (Identity true) (consM (Identity false) (consM (Identity true) (consM (Identity false) nil)))
+                 , ConsM (Identity false) (consM (Identity true) (consM (Identity false) (consM (Identity true) nil)))
+                 , ConsM (Identity false) (consM (Identity false) (consM (Identity false) (consM (Identity false) nil)))
                  ])
               ]
-      exLPBs = [ (exShareSingleton, "exShareSingleton", [ Pair (Identity (Cons (Identity True) nil))
-                                                               (Identity (Cons (Identity True) nil))
-                                                        , Pair (Identity (Cons (Identity False) nil))
-                                                               (Identity (Cons (Identity False) nil))
+      exLPBs = [ (exShareSingleton, "exShareSingleton", [ Pair (Identity (ConsM (Identity true) nil))
+                                                               (Identity (ConsM (Identity true) nil))
+                                                        , Pair (Identity (ConsM (Identity false) nil))
+                                                               (Identity (ConsM (Identity false) nil))
                                                         ])
-               , (exRecList, "exRecList", [ Pair (cons (Identity True) (cons (Identity False) nil))
-                                                (cons (Identity True) (cons (Identity False) nil))
-                                          , Pair (cons (Identity True) (cons (Identity False) nil))
-                                                 (cons (Identity True) (cons (Identity False) nil))
-                                          , Pair (cons (Identity True) (cons (Identity False) nil))
-                                                (cons (Identity True) (cons (Identity False) nil))
+               , (exRecList, "exRecList", [ Pair (consM (Identity true) (consM (Identity false) nil))
+                                                (consM (Identity true) (consM (Identity false) nil))
+                                          , Pair (consM (Identity true) (consM (Identity false) nil))
+                                                 (consM (Identity true) (consM (Identity false) nil))
+                                          , Pair (consM (Identity true) (consM (Identity false) nil))
+                                                (consM (Identity true) (consM (Identity false) nil))
                                           ])
                ]
-      maxName = maximum (map (\(_,name,_) -> length name) exBs ++
-                         map (\(_,name,_) -> length name) exPBs ++
-                         map (\(_,name,_) -> length name) exLBs)
+      maxName = maximum (map (fun (_,name,_) => length name) exBs ++
+                         map (fun (_,name,_) => length name) exPBs ++
+                         map (fun (_,name,_) => length name) exLBs)
       prettyName name = name ++ ": " ++ replicate (maxName - length name) ' '
 
   -- Based on the imported implementation, the annotations for `e` might have to be adapted!
-  mapM_ (\(e,name,v) -> putStr (prettyName name) >> pprint (collectVals (e :: NDShare Bool) == v)) exBs
-  mapM_ (\(e,name,v) -> putStr (prettyName name) >> pprint (collectVals (e :: NDShare (Pair NDShare Bool)) == v)) exPBs
-  mapM_ (\(e,name,v) -> putStr (prettyName name) >> pprint (collectVals (e :: NDShare (List NDShare Bool)) == v)) exLBs
-  mapM_ (\(e,name,v) -> putStr (prettyName name) >>
+  mapM_ (fun (e,name,v) => putStr (prettyName name) >> pprint (collectVals (e :: NDShare Bool) == v)) exBs
+  mapM_ (fun (e,name,v) => putStr (prettyName name) >> pprint (collectVals (e :: NDShare (Pair NDShare Bool)) == v)) exPBs
+  mapM_ (fun (e,name,v) => putStr (prettyName name) >> pprint (collectVals (e :: NDShare (List NDShare Bool)) == v)) exLBs
+  mapM_ (fun (e,name,v) => putStr (prettyName name) >>
     pprint (collectVals (e :: NDShare (Pair NDShare (List NDShare Bool))) == v)) exLPBs
-
-*)
